FixSADRspIFwdM.thy
@@ -1,5 +1,5 @@
 
-theory FixSADRspIFwdM imports BasicInvariants  begin
+theory FixSADRspIFwdM imports BasicInvariants begin
 sledgehammer_params[timeout=10, dont_minimize, "try0" = false]
 lemma HostSADRspIFwdM'_CSTATE_invariant1: shows "CSTATE X (  T [ 1 +=reqresp GO Shared txid] [ 5 sHost= SD] [ 0 -=snpresp  ]) 0 = CSTATE X T 0"
 by simp
