FixSBData.thy
@@ -1,5 +1,5 @@
 
-theory FixSBData imports BasicInvariants  begin
+theory FixSBData imports BasicInvariants begin
 sledgehammer_params[timeout=10, dont_minimize, "try0" = false]
 lemma HostSBData'_devcache_invariant1: shows "(CLEntry.block_state (devcache1 ( T [ 5 sHost= SharedM] [ Dev1 -=d2hdHead ]))) = CLEntry.block_state (devcache1 T)"
 by simp
