FixSharedStore.thy
@@ -1,5 +1,5 @@
 
-theory FixSharedStore imports BasicInvariants  begin
+theory FixSharedStore imports BasicInvariants begin
 sledgehammer_params[timeout=30]
 lemma snps2_SharedStore: shows "snps2 ( T [ 0 +=rdreq RdOwn] [ 0 s= SMAD]) = snps2 T"
 by simp
